Different struct encoding.

handwritten_pulse/SwapStruct.fst
@@ -5,16 +5,82 @@ open Pulse
 module U32 = FStar.UInt32
 module Box = Pulse.Lib.Box
 
-(* The type definitions corresponding to the following struct 
-   are generated in SwapStruct.Types:
+(* The following is to be generated from the C type declaration:
 
 typedef struct _u32_pair_struct {
   uint32_t first;
   uint32_t second;
 } u32_pair_struct;
-
 *)
 
+//1. An abstract type representing a u32_pair_struct
+noeq
+type u32_pair_struct = {
+  first: ref FStar.UInt32.t;
+  second: ref FStar.UInt32.t;
+}
+
+//2. A purely functional specification type for the struct
+[@@erasable]
+noeq
+type u32_pair_struct_spec = {
+  first: FStar.UInt32.t;
+  second: FStar.UInt32.t;
+}
+
+//3. A predicate that relates a u32_pair_struct to its specification
+let u32_pair_struct_pred (x:ref u32_pair_struct) (s:u32_pair_struct_spec) : slprop =
+  exists* (y: u32_pair_struct). (x |-> y) **
+  (y.first |-> s.first) **
+  (y.second |-> s.second)
+
+//4. A utility function to heap u32_pair_struct_allocate and u32_pair_struct_free a u32_pair_struct
+assume val u32_pair_struct_allocated (x: ref u32_pair_struct) : slprop
+
+fn u32_pair_struct_alloc ()
+returns x:ref u32_pair_struct
+ensures u32_pair_struct_allocated x
+ensures exists* v. u32_pair_struct_pred x v
+{ admit () }
+
+fn u32_pair_struct_free (x:ref u32_pair_struct)
+requires u32_pair_struct_allocated x
+requires exists* v. u32_pair_struct_pred x v
+{ admit () }
+
+//5. A ghost function that unfolds the predicate for u32_pair_struct_refs
+ghost fn u32_pair_struct_explode (x:ref u32_pair_struct) (#s:u32_pair_struct_spec)
+requires u32_pair_struct_pred x s
+ensures exists* (v: u32_pair_struct). (x |-> ({first=v.first; second=v.second} <: u32_pair_struct))
+  ** (v.first |-> s.first) ** (v.second |-> s.second)
+{ unfold u32_pair_struct_pred }
+
+//6. Utility functions that convert a reference to the struct to a reference to its fields
+
+// &(x->first)
+fn u32_pair_struct_to_first (x: ref u32_pair_struct) (#first #second: erased _)
+requires x |-> ({ first; second } <: u32_pair_struct)
+requires reveal first |-> 'y
+returns first: ref UInt32.t
+ensures (x |-> ({ first; second } <: u32_pair_struct))
+ensures first |-> 'y
+{ let vx' = !x; rewrite each first as vx'.first; vx'.first }
+
+// &(x->second)
+fn u32_pair_struct_to_second (x: ref u32_pair_struct) (#first #second: erased _)
+requires x |-> ({ first; second } <: u32_pair_struct)
+requires reveal second |-> 'y
+returns second: ref UInt32.t
+ensures (x |-> ({ first; second } <: u32_pair_struct))
+ensures second |-> 'y
+{ let vx' = !x; rewrite each second as vx'.second; vx'.second }
+
+//7. A ghost function that folds the predicate for u32_pair_struct_refs
+ghost
+fn u32_pair_struct_recover (x:ref u32_pair_struct) (#a0 #a1 :erased U32.t)
+requires exists* (y: u32_pair_struct). (x |-> y) ** (y.first |-> a0) ** (y.second |-> a1)
+ensures u32_pair_struct_pred x ({first = a0; second = a1})
+{ fold u32_pair_struct_pred x ({first = a0; second = a1}) }
 
 (*
 RETURNS x
@@ -29,12 +95,15 @@ u32_pair_struct* new_u32_pair_struct ()
 *)
 fn new_u32_pair_struct ()
 requires emp
-returns x:Box.box u32_pair_struct
-ensures exists* (s:u32_pair_struct_spec). SwapStruct.Types.u32_pair_struct_pred (Box.box_to_ref x) s ** pure (s == {first = 0ul; second = 1ul})
+returns x:ref u32_pair_struct
+ensures u32_pair_struct_allocated x
+ensures (u32_pair_struct_pred x { first = 0ul; second = 1ul })
 {
-  let x = SwapStruct.Types.alloc(); //note the translatio of the casted malloc to a typed allocation
-  SwapStruct.Types.set_first (Box.box_to_ref x) 0ul; // assigning to a field of the struct translated to a setter
-  SwapStruct.Types.set_second (Box.box_to_ref x) 1ul; // assigning to a field of the struct translated to a getter
+  let x = u32_pair_struct_alloc(); //note the translation of the casted malloc to a typed allocation
+  u32_pair_struct_explode x;
+  u32_pair_struct_to_first x := 0ul;
+  u32_pair_struct_to_second x := 1ul;
+  u32_pair_struct_recover x;
   x
 }
 
@@ -50,12 +119,14 @@ void swap_fields (u32_pair_struct* x, #s:u32_pair_struct_spec s)
 }
 *)
 fn swap_fields (#s:u32_pair_struct_spec) (x:ref u32_pair_struct)
-requires SwapStruct.Types.u32_pair_struct_pred x s
-ensures exists* (s':u32_pair_struct_spec). SwapStruct.Types.u32_pair_struct_pred x s' ** pure (s' == ({first = s.second; second = s.first}))
+requires u32_pair_struct_pred x s
+ensures exists* (s':u32_pair_struct_spec). u32_pair_struct_pred x s' ** pure (s' == ({first = s.second; second = s.first}))
 {
-  let f1 = SwapStruct.Types.get_first x;
-  SwapStruct.Types.set_first x (SwapStruct.Types.get_second x);
-  SwapStruct.Types.set_second x f1;
+  u32_pair_struct_explode x;
+  let f1 = !(u32_pair_struct_to_first x);
+  u32_pair_struct_to_first x := !(u32_pair_struct_to_second x);
+  u32_pair_struct_to_second x := f1;
+  u32_pair_struct_recover x;
 }
 
 
@@ -94,25 +165,23 @@ void swap_fields_alt (u32_pair_struct* x)
 }
 *)
 fn swap_fields_alt (x:ref u32_pair_struct) (#s:u32_pair_struct_spec)
-requires SwapStruct.Types.u32_pair_struct_pred x s
-ensures exists* (s':u32_pair_struct_spec). SwapStruct.Types.u32_pair_struct_pred x s' ** pure (s' == {first = s.second; second = s.first})
+requires u32_pair_struct_pred x s
+ensures exists* (s':u32_pair_struct_spec). u32_pair_struct_pred x s' ** pure (s' == {first = s.second; second = s.first})
 {
-  let y = SwapStruct.Types.explode x;
-  SwapStruct.Types.u32_pair_struct_refs_pred_unfold y;
-  swap_refs y.first y.second;
-  SwapStruct.Types.u32_pair_struct_refs_pred_fold y;
-  SwapStruct.Types.restore x y;
+  u32_pair_struct_explode x;
+  swap_refs (u32_pair_struct_to_first x) (u32_pair_struct_to_second x);
+  u32_pair_struct_recover x;
 }
 
 (*
 
-void main () 
+void main ()
 {
   u32_pair_struct* x = new_u32_pair_struct ();
-  swap_fields (x);  //translate the heap allocated Box to a ref
-  swap_fields_alt (x); //translate the heap allocated Box to a ref
+  swap_fields (x);
+  swap_fields_alt (x);
   ASSERT (u32_pair_struct_pred x {first = 0ul; second = 1ul});
-  free(x);
+  u32_pair_struct_free(x);
 }
 
 *)
@@ -122,12 +191,11 @@ ensures emp
 {
   let x = new_u32_pair_struct ();
   // Swap fields using the first method
-  swap_fields (Box.box_to_ref x);
+  swap_fields x;
 
-  swap_fields_alt (Box.box_to_ref x);
+  swap_fields_alt x;
 
-  assert (SwapStruct.Types.u32_pair_struct_pred (Box.box_to_ref x) {first = 0ul; second = 1ul});
+  assert (u32_pair_struct_pred x {first = 0ul; second = 1ul});
 
-  SwapStruct.Types.free x;
+  u32_pair_struct_free x;
 }
-  
